Kura/Operation/VxIdentification.lean
@@ -13,28 +13,24 @@ set I am contracting on. This is one way to do it using partitions. -/
 def IsPartitionGraph [CompleteLattice α] (G : Graph α β) : Prop :=
   ∃ P : Partition α, P.parts = V(G)
 
-instance instIsPartitionGraphGraphicVertex : GraphicVertexFunction (fun {β} (G : Graph (Set α) β) ↦
-  G.IsPartitionGraph) where
-  presv_isom G G' h := by
+instance instIsPartitionGraphGraphicVertex [CompleteLattice α] :
+    GraphicVertexFunction (Graph.IsPartitionGraph (α := α)) (Graph.IsPartitionGraph) where
+  invariant h := by
     obtain ⟨f, hf⟩ := h
     rw [eq_iff_iff]
-    refine ⟨fun h ↦ ?_, fun h ↦ ?_⟩
+    refine ⟨fun h ↦ ?_, fun h ↦ ?_⟩ <;>
     · obtain ⟨P, hP⟩ := h
       use P
-      rw [hP]
-      simpa only [HomSys.ofEdgeFun, _root_.bijOn_id] using hf.bijOn_vx
-    · obtain ⟨P, hP⟩ := h
-      use P
-      rw [hP, eq_comm]
-      simpa only [HomSys.ofEdgeFun, _root_.bijOn_id] using hf.bijOn_vx
+      rw [hP, instVxSetGraphicVertex.invariant ⟨f, hf⟩]
+
 
 def Setify (G : Graph α β) : Graph (Set α) β :=
   vxMap G ({·})
 
-def Setify.HasIsom (G : Graph α β) : G ≤↔ G.Setify :=
-  vxMap.HasIsom ({·}) singleton_injective.injOn
+def setify_hasIsom (G : Graph α β) : G ↔ᴳ G.Setify :=
+  vxMap_hasIsom singleton_injective.injOn
 
-lemma Setify.IsPartitionGraph (G : Graph α β) : G.Setify.IsPartitionGraph := by
+lemma setify_isPartitionGraph (G : Graph α β) : G.Setify.IsPartitionGraph := by
   use Partition.discrete V(G)
   ext x
   simp [Partition.discrete, Setify]
@@ -51,19 +47,19 @@ def VxIdentification (G : Graph (Set α) β) (P : Partition (Set (Set α))) :
 variable {P : Partition (Set (Set α))} (hP : ⋃₀ P.parts = V(G))
 
 @[simp]
-lemma vxIdentification_inc₂ : (V(G)xIdentification P).Inc₂ e x y ↔ ∃ x' y',
+lemma vxIdentification_inc₂ : (G.VxIdentification P).Inc₂ e x y ↔ ∃ x' y',
     G.Inc₂ e x' y' ∧ ⋃₀ P.partOf x' = x ∧ ⋃₀ P.partOf y' = y := by
   rw [VxIdentification, vxMap_inc₂]
 
 lemma vxIdentification_inc₂_toMultiset :
-    (V(G)xIdentification P).Inc₂ e x y ↔ (G.toMultiset e).map (⋃₀ P.partOf ·) = {x, y} := by
+    (G.VxIdentification P).Inc₂ e x y ↔ (G.toMultiset e).map (⋃₀ P.partOf ·) = {x, y} := by
   rw [VxIdentification, vxMap_inc₂_toMultiset]
 
 @[simp]
 lemma vxIdentification_toMultiset :
-    (V(G)xIdentification P).toMultiset e = (G.toMultiset e).map (⋃₀ P.partOf ·) := by
+    (G.VxIdentification P).toMultiset e = (G.toMultiset e).map (⋃₀ P.partOf ·) := by
   rw [VxIdentification, vxMap_toMultiset]
 
 @[simp]
-lemma vxIdentification_inc : (V(G)xIdentification P).Inc e x ↔ ∃ y, G.Inc e y ∧ ⋃₀ P.partOf y = x := by
+lemma vxIdentification_inc : (G.VxIdentification P).Inc e x ↔ ∃ y, G.Inc e y ∧ ⋃₀ P.partOf y = x := by
   rw [VxIdentification, vxMap_inc]
